src/Crypto/HKDF/HMAC.dfy
@@ -1,0 +1,82 @@
+include "../Digests.dfy"
+include "../../StandardLibrary/StandardLibrary.dfy"
+
+module {:extern "HMAC"} HMAC {
+  import opened Digests
+  import opened StandardLibrary
+  import opened UInt = StandardLibrary.UInt
+
+  datatype {:extern "CipherParameters"} CipherParameters = KeyParameter(key: array<uint8>)
+
+  class {:extern "HMac"} HMac {
+
+    const algorithm: KeyDerivationAlgorithm
+    ghost var initialized: Option<seq<uint8>>
+
+    // InputSoFar represents the accumulated input as Update calls are made. It is cleared by Reset and DoFinal, though
+    // DoFinal additionally outputs the hash of the accumulated input.
+    ghost var InputSoFar: seq<uint8>
+
+    constructor {:extern} (algorithm: KeyDerivationAlgorithm)
+      requires algorithm != IDENTITY
+      ensures this.algorithm == algorithm
+
+    function method {:extern "GetMacSize"} getMacSize(): int32
+      requires algorithm != IDENTITY
+      ensures getMacSize() == HashLength(algorithm)
+
+    predicate {:axiom} validKey(key: seq<uint8>)
+
+    method {:extern "Init"} init(params: CipherParameters)
+      // The documentation says it can throw "InvalidKeyException - if the given key is inappropriate for
+      // initializing this MAC", which I have interpreted to mean the following precondition:
+      //requires key.algorithm == algorithm
+      requires params.KeyParameter?
+      modifies this
+      ensures
+        var key := match params case KeyParameter(key) => key;
+        match initialized { case Some(k) => validKey(k) && key[..] == k case None => false }
+      ensures InputSoFar == []
+
+    method {:extern "Reset"} reset()
+      requires initialized.Some?
+      modifies `InputSoFar
+      ensures InputSoFar == []
+
+    method {:extern "Update"} updateSingle(input: uint8)
+      requires initialized.Some?
+      modifies this
+      ensures unchanged(`initialized)
+      ensures InputSoFar == old(InputSoFar) + [input]
+
+    method {:extern "BlockUpdate"} update(input: array<uint8>, inOff: int32, len: int32)
+      requires initialized.Some?
+      requires inOff >= 0
+      requires len >= 0
+      requires input.Length < INT32_MAX_LIMIT
+      requires inOff as int + len as int <= input.Length
+      modifies `InputSoFar
+      ensures InputSoFar == old(InputSoFar) + input[inOff..inOff+len]
+
+    method {:extern "DoFinal"} doFinal(output: array<uint8>, outOff: int32) returns (retVal: int32)
+      requires initialized.Some?
+      requires algorithm != IDENTITY
+      requires outOff >= 0
+      requires outOff as int + getMacSize() as int <= output.Length
+      requires |Hash(algorithm, initialized.get, InputSoFar)| == getMacSize() as int
+      requires output.Length < INT32_MAX_LIMIT
+      modifies `InputSoFar, output
+      ensures output[..] == old(output[..outOff]) + old(Hash(algorithm, initialized.get, InputSoFar)) + old(output[outOff + getMacSize()..])
+      ensures output.Length == old(output.Length)
+      ensures InputSoFar == []
+
+    method updateAll(input: array<uint8>)
+      requires initialized.Some?
+      requires input.Length < INT32_MAX_LIMIT
+      modifies `InputSoFar
+      ensures InputSoFar == old(InputSoFar) + input[..]
+    {
+      update(input, 0, input.Length as int32);
+    }
+  }
+}
